src/impl/TLS13.Impl.Driver.PairingNoTailNormalized.fsti
@@ -207,6 +207,16 @@ let paired_no_tail_role_local_start_spine16
   PNTSS.server_no_tail_start_spine16 server
 
 noextract
+let paired_no_tail_role_local_start_and_final_witnesses16
+  (client:CS.connection_state)
+  (server:CS.connection_state)
+  : prop =
+  PNTCS.client_no_tail_start_spine client /\
+  PNTCS.client_no_tail_final_model_witnesses client /\
+  PNTSS.server_no_tail_start_spine16 server /\
+  PNTSS.server_no_tail_final_model_witnesses server
+
+noextract
 let paired_no_tail_role_local_client_two_handshake_installs_server_start_spine16
   (client:CS.connection_state)
   (server:CS.connection_state)
@@ -358,6 +368,28 @@ val lemma_clean16_no_tail_valid_byte_traces_role_local_start_spine16
           server_received
           server_sent)
       (ensures paired_no_tail_role_local_start_spine16 client server)
+
+val lemma_clean16_no_tail_valid_byte_traces_role_local_start_and_final_witnesses16
+  (client_initial:CS.connection_state)
+  (server_initial:CS.connection_state)
+  (client:CS.connection_state)
+  (server:CS.connection_state)
+  (client_received:B.bytes)
+  (client_sent:B.bytes)
+  (server_received:B.bytes)
+  (server_sent:B.bytes)
+  : Lemma
+      (requires
+        paired_supported_no_tail_valid_byte_traces_clean16
+          client_initial
+          server_initial
+          client
+          server
+          client_received
+          client_sent
+          server_received
+          server_sent)
+      (ensures paired_no_tail_role_local_start_and_final_witnesses16 client server)
 
 val lemma_clean16_no_tail_valid_byte_traces_role_local_client_two_handshake_installs_server_start_spine16
   (client_initial:CS.connection_state)
